cpp

protocol.v
@@ -74,6 +74,7 @@ Class CBC_protocol_eq :=
       about_state : StrictlyComparable state;
       state0 : state;
       state_eq : state -> state -> Prop;
+      state_eq_equiv :> Equivalence state_eq;
       state_union : state -> state -> state;
       state_union_comm : forall s1 s2, state_eq (state_union s1 s2) (state_union s2 s1);
       (** Reachability relation **) 
@@ -94,6 +95,1508 @@ Class CBC_protocol_eq :=
       about_prot_state : forall s1 s2, prot_state s1 -> prot_state s2 ->
                                   (equivocation_weight (state_union s1 s2) <= proj1_sig t)%R -> prot_state (state_union s1 s2);
    }.
+
+Class CBC_protocol_eq_specific `{CBC_protocol_eq} :=
+  {
+    two_senders : exists (v1 v2 : validators), v1 <> v2;
+
+    (* Being duplicate-free means something different across protocols *)
+    state_nodup : state -> Prop;
+    prot_state_nodup : forall (s : state), prot_state s ->
+                                      state_nodup s;
+    nodup_state_reach : forall (s : state), state_nodup s ->
+                                       forall (s' : state), reach s' s ->
+                                                       state_nodup s';
+    protocol_state_incl : forall (s : state), prot_state s ->
+                                         forall (s' : state),
+                                           state_nodup s' ->
+                                           reach s' s ->
+                                           prot_state s';
+    (* Notion of messages *) 
+    message : Type;
+    about_message : StrictlyComparable message;
+
+
+    get_messages : state -> list message;
+    justification : message -> state;
+    sender : message -> validators;
+    add_message : message -> state -> state;
+
+    prot_state_extend_nodup : forall (s : state) (msg : message),
+        justification msg = s -> state_nodup (add_message msg s);
+    in_state : message -> state -> Prop;
+    in_state_correct : forall (msg : message) (s : state),
+        in_state msg s <-> In msg (get_messages s);
+    in_state_morphism : forall (s1 s2 : state), reach s1 s2 ->
+                                           forall (msg : message),
+                                             in_state msg s1 ->
+                                             in_state msg s2;
+    add_message_in_state : forall (msg : message) (s : state), in_state msg (add_message msg s);
+    add_message_get_messages_iff : forall sigma msg,
+        get_messages (add_message msg sigma) = msg :: get_messages sigma;
+    in_state_add_message_iff : forall msg msg' sigma',
+        in_state msg (add_message msg' sigma') <->
+        msg = msg' \/ in_state msg sigma';
+    add_message_rel : forall (msg : message) (s : state), reach s (add_message msg s);
+
+    (* Message-specific equivocation function *)
+    equivocating_messages : message -> message -> bool;
+    equivocating_messages_comm : forall msg1 msg2, equivocating_messages msg1 msg2 = equivocating_messages msg2 msg1; 
+    equivocating_messages_correct : forall msg1 msg2, equivocating_messages msg1 msg2 = true <-> (msg1 <> msg2 /\
+                                                                                           sender msg1 = sender msg2 /\
+                                                                                          ~ in_state msg1 (justification msg2) /\
+                                                                                          ~ in_state msg2 (justification msg1));
+    
+
+    (* Now we need to figure out exactly what we need to know about the next equivocation state *) 
+    next_equivocation_state : state -> validators -> validators -> state;
+    next_equivocation_state_incl : forall (j : state) (v v' : validators), reach j (next_equivocation_state j v v');
+    
+    next_equivocation_state_nodup : forall j v v',
+        state_nodup (next_equivocation_state j v v'); 
+
+    (* This is apparently not enough - we also need to know that we can create a horn from our next equivocation state. *)
+    next_equivocation_state_horn : forall (j : state) (v v' : validators), exists msg1 msg2 msg3,
+          next_equivocation_state j v v' = add_message msg3 (add_message msg2 (add_message msg1 j)) /\
+          equivocating_messages msg2 msg3 = true /\
+          sender msg2 = v /\ 
+          sender msg1 = v' /\
+          justification msg1 = j /\
+          prot_state (add_message msg3 j) /\
+          prot_state (add_message msg2 (add_message msg1 j)); 
+  }.
+
+Definition equivocating_messages_prop `{CBC_protocol_eq_specific} :=
+  fun (msg1 msg2 : message) => msg1 <> msg2 /\
+                            sender msg1 = sender msg2 /\
+                            ~ in_state msg1 (justification msg2) /\
+                            ~ in_state msg2 (justification msg1).
+
+Lemma equivocating_messages_correct' `{CBC_protocol_eq_specific} : forall msg1 msg2,
+    equivocating_messages msg1 msg2 = false <-> ~ equivocating_messages_prop msg1 msg2. 
+Proof.
+  intros. 
+  apply mirror_reflect_curry.
+  apply equivocating_messages_correct.
+Qed. 
+                                
+Definition equivocating_in_state `{CBC_protocol_eq_specific} (msg : message) (sigma : state) : bool :=
+  existsb (equivocating_messages msg) (get_messages sigma).
+
+Definition equivocating_in_state_prop `{CBC_protocol_eq_specific} :=
+  fun (msg : message) (s : state) =>
+    exists (msg' : message), in_state msg' s /\ equivocating_messages_prop msg msg'.
+
+Lemma equivocating_in_state_correct `{CBC_protocol_eq_specific} :
+  forall msg s, equivocating_in_state msg s = true <-> equivocating_in_state_prop msg s.
+Proof.
+  rename H into elephant.
+  rename H0 into squirrel.
+  intros msg s.
+  split; intro H.
+  - unfold equivocating_in_state in H.
+    rewrite existsb_exists in H.
+    destruct H as [msg' [H_in H_equiv]].
+    exists msg'. split.
+    apply in_state_correct. assumption.
+    unfold equivocating_messages_prop.
+    rewrite <- equivocating_messages_correct. assumption.
+  - destruct H as [msg' [H_in H_equiv]].
+    apply existsb_exists.
+    exists msg'; split. apply in_state_correct. assumption.
+    rewrite equivocating_messages_correct. assumption.
+Qed.
+
+Lemma equivocating_in_state_correct' `{CBC_protocol_eq_specific} :
+  forall msg s, equivocating_in_state msg s = false <-> ~ equivocating_in_state_prop msg s.
+Proof.
+  intros. 
+  apply mirror_reflect_curry.
+  exact equivocating_in_state_correct.
+Qed.
+
+Lemma equivocating_in_state_incl `{CBC_protocol_eq_specific} :
+  forall sigma sigma',
+  reach sigma sigma' ->
+  forall msg,
+    equivocating_in_state_prop msg sigma ->
+    equivocating_in_state_prop msg sigma'.
+Proof.
+  intros. destruct H2 as [x [Hin Heq]]. exists x.
+  split; try assumption.
+  now apply in_state_morphism with sigma. 
+Qed.
+
+Lemma non_equivocating_messages_sender `{CBC_protocol_eq_specific} : forall msg1 msg2,
+  sender msg1 <> sender msg2 ->
+  equivocating_messages msg1 msg2 = false.
+Proof.
+  intros msg1 msg2 Hneq. simpl in Hneq.
+Admitted. 
+
+Lemma equivocating_in_state_not_seen `{CBC_protocol_eq_specific} :
+  forall (msg : message) (sigma : state),
+  ~ In (sender msg) (set_map (@compare_eq_dec validators (@compare validators about_validators) (@compare_strictorder validators about_validators)) sender (get_messages sigma)) ->
+  ~ equivocating_in_state_prop msg sigma.  
+Proof.
+  intros msg sigma Hnin. rewrite set_map_exists in Hnin. simpl in Hnin.
+  rewrite <- equivocating_in_state_correct'. 
+  apply existsb_forall.
+  intros msg' Hin.
+  apply non_equivocating_messages_sender. simpl.
+  intro Heq. subst. apply Hnin.
+  exists msg'. split; try assumption. symmetry; assumption.
+Qed.
+
+Lemma equivocating_messages_prop_swap `{CBC_protocol_eq_specific} : forall msg1 msg2,
+  equivocating_messages_prop msg1 msg2 <-> equivocating_messages_prop msg2 msg1.
+Proof.
+  intros msg1 msg2.
+  unfold equivocating_messages_prop.
+  do 2 rewrite <- equivocating_messages_correct.
+  split; intro H_true;
+  now rewrite equivocating_messages_comm.
+Qed.
+
+Definition equivocating_senders `{CBC_protocol_eq_specific} (sigma : state) : set validators :=
+  set_map (@compare_eq_dec validators (@compare validators about_validators) (@compare_strictorder validators about_validators)) sender
+    (filter (fun msg => equivocating_in_state msg sigma)
+      (get_messages sigma)).
+
+Definition equivocating_senders_prop `{CBC_protocol_eq_specific} (s : state) (lv : set validators) :=
+  forall v, In v lv <-> exists msg, in_state msg s /\ sender msg = v /\ equivocating_in_state_prop msg s. 
+
+Lemma equivocating_senders_correct`{CBC_protocol_eq_specific} : forall s,
+    equivocating_senders_prop s (equivocating_senders s).
+Proof.
+  rename H into elephant.
+  rename H0 into squirrel.
+  intros s v; split; intro H. 
+  - (* Left direction *)
+    apply set_map_exists in H.
+    destruct H as [msg [H_in H_sender]].
+    exists msg.
+    apply filter_In in H_in.
+    destruct H_in. repeat split; try assumption.
+    apply in_state_correct in H.
+    assumption.
+    rewrite <- equivocating_in_state_correct.
+    assumption.
+  - destruct H as [msg [H_in [H_sender H_equiv]]]. 
+    unfold equivocating_senders.
+    rewrite <- H_sender.
+    apply set_map_in.
+    rewrite filter_In. split.
+    apply in_state_correct. assumption.
+    rewrite equivocating_in_state_correct.
+    assumption.
+Qed.
+
+Lemma equivocating_senders_incl `{CBC_protocol_eq_specific} : forall sigma sigma',
+  reach sigma sigma' ->
+  incl (equivocating_senders sigma) (equivocating_senders sigma').
+Proof.
+  intros.
+  apply set_map_incl.
+  apply incl_tran with (filter (fun msg : message => equivocating_in_state msg sigma) (get_messages sigma')).
+  - apply filter_incl.
+    intros msg H_msg_in.
+    apply in_state_correct.
+    apply in_state_correct in H_msg_in.
+    now apply in_state_morphism with sigma. 
+  - intros v H_in.
+    rewrite filter_In in *.
+    destruct H_in. split. assumption.
+    rewrite equivocating_in_state_correct in *.
+    now apply equivocating_in_state_incl with sigma.
+Qed.
+
+Lemma non_equivocating_messages_extend `{CBC_protocol_eq_specific} : forall msg sigma1,
+    In msg (get_messages sigma1) ->
+    forall msg',
+      justification msg' = sigma1 -> 
+      equivocating_messages msg msg' = false.
+Proof.
+  intros msg; intros.
+  apply equivocating_messages_correct'. 
+  intros H_absurd.
+  destruct H_absurd as [H_msg [H_sender [H_just_l H_just_r]]].
+  subst.
+  apply in_state_correct in H1.
+  contradiction.
+Qed.
+
+Lemma equivocating_senders_extend `{CBC_protocol_eq_specific} :
+  forall sigma msg,
+    justification msg = sigma ->
+    equivocating_senders (add_message msg sigma) = equivocating_senders sigma.
+Proof.
+  rename H into elephant. rename H0 into squirrel.
+  unfold equivocating_senders. intros. 
+  (* Why doesn't the suff tactic work *)
+  assert (H_suff : 
+    (filter (fun msg : message => equivocating_in_state msg (add_message msg sigma))
+      (get_messages (add_message msg sigma))) = 
+    (filter (fun msg : message => equivocating_in_state msg sigma)
+            (get_messages sigma))); try (rewrite H_suff; reflexivity).
+  rewrite add_message_get_messages_iff. 
+  simpl.
+  assert
+    (Hequiv : equivocating_in_state msg (add_message msg sigma) = false)
+  ; try rewrite Hequiv.
+  { apply existsb_forall. intros.
+    rewrite equivocating_messages_comm.
+    apply in_state_correct in H0.
+    rewrite in_state_add_message_iff in H0.
+    destruct H0 as [Heq | Hin].
+    - subst.
+      apply not_true_iff_false.
+      intro H_absurd.
+      rewrite equivocating_messages_correct in H_absurd.
+      destruct H_absurd; tauto. 
+    - apply in_state_correct in Hin.
+      now apply non_equivocating_messages_extend with sigma. 
+  }
+  apply filter_eq_fn. intros. unfold equivocating_in_state. split; intros
+  ; apply existsb_exists in H1; apply existsb_exists
+  ; destruct H1 as [msg' [Hin Hmsg]]; exists msg'; split; try assumption.
+  - rewrite add_message_get_messages_iff in Hin.
+    destruct Hin as [Heq | Hin]; try assumption.
+    exfalso. subst.
+    apply equivocating_messages_correct in Hmsg.
+    destruct Hmsg as [H_absurd _].
+    apply H_absurd. auto. 
+  - apply in_state_correct.
+    rewrite in_state_add_message_iff.
+    right. apply in_state_correct. assumption.
+  - f_equal.
+    rewrite add_message_get_messages_iff. 
+    simpl.
+     assert
+    (Hequiv : equivocating_in_state msg (add_message msg sigma) = false)
+  ; try rewrite Hequiv.
+  { apply existsb_forall. intros.
+    rewrite equivocating_messages_comm.
+    apply in_state_correct in H0.
+    rewrite in_state_add_message_iff in H0.
+    destruct H0 as [Heq | Hin].
+    - subst.
+      apply not_true_iff_false.
+      intro H_absurd.
+      rewrite equivocating_messages_correct in H_absurd.
+      destruct H_absurd; tauto. 
+    - apply in_state_correct in Hin.
+      now apply non_equivocating_messages_extend with sigma. 
+  }
+    apply filter_eq_fn. intros. unfold equivocating_in_state. split; intros
+  ; apply existsb_exists in H1; apply existsb_exists
+  ; destruct H1 as [msg' [Hin Hmsg]]; exists msg'; split; try assumption.
+  rewrite add_message_get_messages_iff in Hin.
+  destruct Hin as [Heq | Hin]; try assumption.
+  exfalso. subst.
+  assert (H_useful := non_equivocating_messages_extend a (justification msg') H0 msg' eq_refl). 
+  rewrite Hmsg in H_useful.
+  inversion H_useful.
+  apply in_state_correct.
+  rewrite in_state_add_message_iff.
+  right. apply in_state_correct. assumption. 
+Qed.
+
+(* Now let's see if we can define the fault weight of a state parametrically *)
+Definition sum_weights `{CBC_protocol_eq_specific} (l : list validators) : R :=
+  fold_right (fun v r => (proj1_sig (weight v) + r)%R) 0%R l. 
+
+Definition fault_weight_state `{CBC_protocol_eq_specific} (sigma : state) : R :=
+  sum_weights (equivocating_senders sigma). 
+
+Lemma sum_weights_in `{CBC_protocol_eq_specific} : forall v vs,
+  NoDup vs ->
+  In v vs ->
+  sum_weights vs = (proj1_sig (weight v) + sum_weights (set_remove (@compare_eq_dec validators (@compare validators about_validators) (@compare_strictorder validators about_validators)) v vs))%R.
+Proof.
+  rename H into elephant; rename H0 into squirrel.
+  induction vs; intros; inversion H0; subst; clear H0.
+  - inversion H; subst; clear H. simpl. apply Rplus_eq_compat_l.
+    destruct (eq_dec_left (@compare_eq_dec validators (@compare validators about_validators) (@compare_strictorder validators about_validators)) v). rewrite H. reflexivity.
+  - inversion H; subst; clear H. simpl. assert (Hav := H3). apply (in_not_in _ _ _ _ H1) in Hav.
+    destruct (compare_eq_dec v a); try (exfalso; apply Hav; assumption). simpl.
+    rewrite <- Rplus_assoc. rewrite (Rplus_comm (proj1_sig (weight v)) (proj1_sig (weight a))). rewrite Rplus_assoc. 
+    apply Rplus_eq_compat_l. apply IHvs; assumption.
+Qed.
+
+Lemma sum_weights_incl `{CBC_protocol_eq_specific} : forall vs vs',
+  NoDup vs ->
+  NoDup vs' ->
+  incl vs vs' ->
+  (sum_weights vs <= sum_weights vs')%R.
+Proof.
+  rename H into elephant; rename H0 into squirrel.
+  intros vs vs'. generalize dependent vs.
+  induction vs'; intros.
+  - apply incl_empty in H1; subst. apply Rle_refl.
+  - inversion H0; subst; clear H0.
+    destruct (in_dec (@compare_eq_dec validators (@compare validators about_validators) (@compare_strictorder validators about_validators)) a vs).
+    + apply sum_weights_in in i. rewrite i. simpl.
+      apply Rplus_le_compat_l. apply IHvs'.
+      * apply (set_remove_nodup compare_eq_dec a). assumption.
+      * assumption.
+      * intros x Hrem. apply set_remove_iff in Hrem; try assumption.
+        destruct Hrem as [Hin Hxa].
+        apply H1 in Hin. destruct Hin; try assumption.
+        exfalso; subst. apply Hxa. reflexivity.
+      * assumption.
+    + simpl. apply Rle_trans with (sum_weights vs').
+      * apply IHvs'; try assumption.
+        intros x Hin. apply H1 in Hin as Hin'. destruct Hin'; try assumption.
+        exfalso; subst. apply n. assumption.
+      * rewrite <- Rplus_0_l at 1. apply Rplus_le_compat_r. left. destruct weight. simpl. auto. 
+Qed.
+
+Lemma fault_weight_state_incl `{CBC_protocol_eq_specific} : forall sigma sigma',
+  reach sigma sigma' ->
+  (fault_weight_state sigma <= fault_weight_state sigma')%R.
+Proof.
+  intros. apply sum_weights_incl; try apply set_map_nodup.
+  apply equivocating_senders_incl. assumption.
+Qed.
+
+Definition incl_messages `{CBC_protocol_eq_specific} (s1 s2 : state) : Prop :=
+  incl (get_messages s1) (get_messages s2).
+
+(* Estimator approval condition *) 
+Definition valid_estimate `{CBC_protocol_eq_specific} (c : consensus_values) (sigma : state) : Prop :=
+  E sigma c.
+
+(* The not overweight condition *)
+Definition not_heavy `{CBC_protocol_eq_specific} (sigma : state) : Prop :=
+  (fault_weight_state sigma <= proj1_sig t)%R.
+
+(* States following Empty states are never overweight *) 
+Lemma not_heavy_single `{CBC_protocol_eq_specific} :
+  forall msg, not_heavy (add_message msg state0).
+Proof.
+  intros msg. 
+  unfold not_heavy, fault_weight_state, equivocating_senders.
+  simpl. unfold equivocating_in_state. simpl.
+  unfold equivocating_messages. 
+Abort. 
+
+(* If a state is not overweight, none of its subsets are *) 
+Lemma not_heavy_subset `{CBC_protocol_eq_specific} : forall s s',
+  reach s s' ->
+  not_heavy s' ->
+  not_heavy s.
+Proof.
+  red.
+  intros.
+  apply Rle_trans with (fault_weight_state s'); try assumption.
+  apply fault_weight_state_incl; assumption.
+Qed.
+
+Lemma equivocating_in_state_extend `{CBC_protocol_eq_specific} :
+  forall s msg,
+    justification msg = s -> 
+    ~ equivocating_in_state_prop msg s.
+Proof. 
+  intros s msg H_just H_absurd.
+  destruct H_absurd as [msg' [H_in H_equiv]].
+  apply in_state_correct in H_in. 
+  assert (H_useful := non_equivocating_messages_extend msg' s H_in). 
+  spec H_useful msg H_just.
+  rewrite equivocating_messages_correct' in H_useful.
+  rewrite equivocating_messages_prop_swap in H_equiv.
+  contradiction.
+Qed.
+
+Definition pstate_light `{CBC_protocol_eq_specific} : Type := {s : state | prot_state s}. 
+Definition pstate_light_proj1 `{CBC_protocol_eq_specific} (p : pstate_light) : state :=
+  proj1_sig p. 
+Coercion pstate_light_proj1 : pstate_light >-> state.
+
+Definition pstate_light_rel `{CBC_protocol_eq_specific} : pstate_light -> pstate_light -> Prop :=
+  fun p1 p2 => reach (pstate_light_proj1 p1) (pstate_light_proj1 p2).
+
+Definition non_trivial_pstate_light `{CBC_protocol_eq_specific} (P : pstate_light -> Prop) :=
+  (exists (s1 : pstate_light), forall (s : pstate_light), pstate_light_rel s1 s -> P s)
+  /\
+  (exists (s2 : pstate_light), forall (s : pstate_light), pstate_light_rel s2 s -> (P s -> False)).
+
+Lemma Rtotal_le_gt : forall x y,
+  (x <= y)%R \/ (x > y)%R.
+Proof.
+  intros.
+  destruct (Rtotal_order x y) as [Hlt | [Heq | Hgt]].
+  - left. unfold Rle. left. assumption.
+  - left. unfold Rle. right. assumption.
+  - right. assumption.
+Qed.
+
+Lemma next_equivocation_state_keeps_messages `{CBC_protocol_eq_specific} :
+  forall (j : state) (v v' : validators) (msg : message),
+    In msg (get_messages j) ->
+    In msg (get_messages (next_equivocation_state j v v')). 
+Proof.
+  intros.
+  assert (H_useful := next_equivocation_state_incl j v v').
+  rewrite <- in_state_correct in *.
+  now apply in_state_morphism with j.  
+Qed.
+
+Lemma next_equivocation_state_keeps_equivocators `{CBC_protocol_eq_specific} :
+  forall (j : state) (v v' v0 : validators),
+    In v0 (equivocating_senders j) ->
+    In v0 (equivocating_senders (next_equivocation_state j v v')). 
+Proof.
+  intros.
+  assert (H_incl := equivocating_senders_incl).
+  spec H_incl j (next_equivocation_state j v v') (next_equivocation_state_incl j v v').
+  now apply H_incl. 
+Qed.
+
+Lemma next_equivocation_state_keeps_equivocating_messages `{CBC_protocol_eq_specific} :
+  forall (j : state) (v v' : validators) (msg : message),
+    equivocating_in_state_prop msg j ->
+    equivocating_in_state_prop msg (next_equivocation_state j v v'). 
+Proof.
+  intros.
+  assert (H_incl := equivocating_in_state_incl).
+  spec H_incl j (next_equivocation_state j v v') (next_equivocation_state_incl j v v').
+  now apply H_incl. 
+Qed.
+
+(* It just occurred to me that we don't need to be overly specific about how we create this next equivocation state. *) 
+
+
+Lemma equivocating_senders_sorted_extend `{CBC_protocol_eq_specific} :
+  forall s msg,
+    justification msg = s -> 
+    set_eq (equivocating_senders s)
+           (equivocating_senders (add_message msg s)). 
+Proof.
+  intros.
+  assert (H_useful := equivocating_senders_extend s msg).
+  rewrite <- H_useful.
+  apply set_eq_refl. 
+  assumption.
+Qed.
+
+Lemma set_eq_nodup_sum_weight_eq `{CBC_protocol_eq_specific} :
+  forall (lv1 lv2 : list validators),
+    NoDup lv1 ->
+    NoDup lv2 ->
+    set_eq lv1 lv2 ->
+    sum_weights lv1 = sum_weights lv2. 
+Proof.
+  intros lv1 lv2 H_nodup1 H_nodup2 [H_eq_l H_eq_r].
+  assert (H_useful := sum_weights_incl lv1 lv2 H_nodup1 H_nodup2 H_eq_l).
+  assert (H_useful' := sum_weights_incl lv2 lv1 H_nodup2 H_nodup1 H_eq_r).
+  now apply Rle_antisym. 
+Qed.
+
+Lemma equivocating_senders_fault_weight_eq `{CBC_protocol_eq_specific} :
+  forall s1 s2,
+    set_eq (equivocating_senders s1) (equivocating_senders s2) ->
+    fault_weight_state s1 = fault_weight_state s2. 
+Proof.
+  intros s1 s2 H_eq. 
+  apply set_eq_nodup_sum_weight_eq; try apply set_map_nodup.
+  assumption.
+Qed.
+
+Require Import Classical. 
+
+Lemma add_already_equivocating_sender `{CBC_protocol_eq_specific} :
+  forall (s : state),
+    prot_state s ->
+    forall (msg : message),
+      In (sender msg) (equivocating_senders s) ->
+        set_eq (equivocating_senders s)
+               (equivocating_senders (add_message msg s)). 
+Proof.
+  intros s about_s msg H_in.
+  split; intros v H_v_in.
+  - unfold equivocating_senders.
+    apply set_map_exists in H_v_in.
+    destruct H_v_in as [msg' [H_v_in H_msg'_sender]].
+    apply filter_In in H_v_in.
+    rewrite <- H_msg'_sender.
+    apply set_map_in.
+    apply filter_in. 
+    rewrite add_message_get_messages_iff. right. 
+    tauto.
+    rewrite equivocating_in_state_correct.
+    destruct H_v_in.
+    rewrite equivocating_in_state_correct in H2.
+    destruct H2 as [msg'_partner H2].
+    red. exists msg'_partner. split.
+    destruct H2.
+    rewrite in_state_correct.
+    rewrite add_message_get_messages_iff.
+    apply in_state_correct in H2. right; assumption.
+    tauto.
+  - destruct (classic (v = sender msg)).
+    + subst. assumption. 
+    + unfold equivocating_senders in H_v_in.
+      apply set_map_exists in H_v_in.
+      destruct H_v_in as [msg' [H_v_in H_msg'_sender]].
+      apply filter_In in H_v_in.
+      destruct H_v_in as [H_v_in H_equiv].
+      rewrite equivocating_in_state_correct in H_equiv.
+      destruct H_equiv as [msg'_partner [H_msg'_partner_in H_equiv]].
+      rewrite <- H_msg'_sender.
+      apply set_map_in.
+      apply filter_in.
+      rewrite add_message_get_messages_iff in H_v_in.
+      destruct H_v_in.
+      subst.
+      contradiction.
+      assumption.
+      rewrite equivocating_in_state_correct.
+      exists msg'_partner.
+      split.
+      apply in_state_correct in H_msg'_partner_in.
+      rewrite add_message_get_messages_iff in H_msg'_partner_in.
+      destruct H_msg'_partner_in.
+      subst. destruct H_equiv.
+      destruct H1. tauto.
+      apply in_state_correct. 
+      assumption. assumption.
+Qed.
+
+Lemma senders_fault_weight_eq `{CBC_protocol_eq_specific} :
+  forall lv1 lv2,
+    NoDup lv1 ->
+    NoDup lv2 ->
+    set_eq lv1 lv2 ->
+    sum_weights lv1 = sum_weights lv2. 
+Proof.
+  rename H into elephant.
+  rename H0 into squirrel.
+  induction lv1 as [|hd tl IHlv1]; intros lv2 H_lv1 H_lv2 H_eq.
+  - destruct lv2.
+    reflexivity.
+    inversion H_eq.
+    spec H0 v (in_eq v lv2).
+    inversion H0.
+  - simpl.
+    (* hd must be in duplicate-free lv2 *)
+    spec IHlv1 (set_remove (@compare_eq_dec validators (@compare validators about_validators) (@compare_strictorder validators about_validators)) hd lv2).
+    spec IHlv1.
+    apply NoDup_cons_iff in H_lv1. tauto.
+    spec IHlv1.
+    now apply set_remove_nodup.
+    spec IHlv1.
+    replace tl with (set_remove (@compare_eq_dec validators (@compare validators about_validators) (@compare_strictorder validators about_validators)) hd (hd :: tl)). 
+    apply set_eq_remove; try assumption.
+    now rewrite set_remove_first.
+    (* Now. *) 
+    rewrite IHlv1.
+    symmetry.
+    apply sum_weights_in. assumption.
+    destruct H_eq as [H_eq _].
+    spec H_eq hd (in_eq hd tl). assumption.
+Qed.
+
+Lemma set_add_ignore {X} `{StrictlyComparable X} :
+  forall (l : list X) (x : X),
+    In x l ->
+    set_add compare_eq_dec x l = l. 
+Proof.
+  induction l as [|hd tl IHl]; intros x H_in. 
+  - inversion H_in.
+  - inversion H_in.
+    + subst. simpl.
+      destruct (compare_eq_dec x x). 
+      reflexivity.
+      contradiction.
+    + spec IHl x H0. simpl.
+      destruct (compare_eq_dec x hd).
+      reflexivity.
+      rewrite IHl. reflexivity.
+Qed.
+
+Lemma add_equivocating_sender `{CBC_protocol_eq_specific} :
+  forall (s : state),
+    prot_state s ->
+    forall (msg : message),
+      (exists msg',
+          in_state msg' s /\
+          equivocating_messages_prop msg msg') ->
+      set_eq (equivocating_senders (add_message msg s))
+             (set_add (@compare_eq_dec validators (@compare validators about_validators) (@compare_strictorder validators about_validators)) (sender msg) (equivocating_senders s)).
+Proof.
+  (* Because we're using set_add, we don't need to care about whether (sender msg) is already in (equivocating_senders s) *) 
+  intros s about_s msg [msg' [H_in H_equiv]]. 
+  destruct (classic (In msg (get_messages s))) as [H_msg_in | H_msg_out].
+  - (* In the case that msg is already in s, *)
+    (* Adding it does nothing to the state *)
+    assert (H_ignore := @set_add_ignore message about_message (get_messages s) msg H_msg_in).
+    simpl in *.
+    admit. 
+(*     replace (add_message msg s) with (msg :: get_messages s). rewrite <- H_ignore.
+    (* Adding the sender should do nothing to (equivocating_senders s) *) 
+    split.
+    + intros v0 H_mem.
+      (* The following is winding and painful *) 
+      unfold equivocating_senders in H_mem.
+      rewrite set_map_exists in H_mem.
+      destruct H_mem as [msg0 [H0_in H0_sender]].
+      rewrite filter_In in H0_in.
+      assert (H_senders := equivocating_senders_correct s). 
+      red in H_senders.
+      destruct H0_in as [H0_in H0_equiv].
+      apply set_add_iff. 
+      destruct (classic (msg = msg0)).
+      * subst.
+        left; reflexivity. 
+      * inversion H0_in. contradiction.
+        clear H0_in.
+        rewrite H_ignore in *.
+        rewrite equivocating_in_state_correct in H0_equiv. 
+        destruct H0_equiv as [msg0_partner [H0_equivl H0_equivr]].
+        inversion H0_equivl.
+        subst. left.
+        destruct H0_equivr. tauto.
+        right.
+        subst.
+        spec H_senders (sender msg0).
+        apply H_senders.
+        exists msg0_partner. 
+        repeat split. assumption. red in H0_equivr; symmetry; tauto.
+        exists msg0. split; try assumption.
+        apply equivocating_messages_prop_swap.
+        assumption. 
+    + intros v0 H_mem.
+      (* The following will also be winding and painful *)
+      destruct (classic (v0 = sender msg)).
+      * subst.
+        clear H_mem.
+        apply set_map_in.
+        apply filter_in.
+        apply in_eq. 
+        rewrite equivocating_in_state_correct.
+        exists msg'. split; try assumption.
+        right; rewrite H_ignore; assumption. 
+      * rewrite set_add_iff in H_mem.
+        destruct H_mem.
+        contradiction. rewrite H_ignore in *.
+        assert (H_goal := equivocating_senders_incl s (msg :: s)). spec H_goal. right; now apply incl_refl.
+        now apply H_goal. 
+  - (* In the case that msg is not already in s, *)
+    (* For all we know (sender msg) could already be in (equivocating_senders s) *)  
+    destruct (classic (In (sender msg) (equivocating_senders s))).
+    + (* If (sender msg) is already in there, then adding it again does nothing *)
+      assert (H_ignore : set_eq (set_add compare_eq_dec (sender msg) (equivocating_senders s)) (equivocating_senders s)).
+      {  split; intros v H_v_in. 
+         apply set_add_iff in H_v_in.
+         destruct H_v_in.
+         subst; assumption.
+         assumption.
+         apply set_add_iff. right; assumption. }
+      apply set_eq_comm in H_ignore. 
+      eapply set_eq_tran. 
+      2 : exact H_ignore.
+      apply set_eq_comm.
+      now apply add_already_equivocating_sender.
+    + (* If (sender msg) is not already in there *)
+      split; intros.  
+      * intros v0 H_in0.
+        destruct (classic (v0 = sender msg)). 
+        ** subst.
+           apply set_add_iff.
+           tauto.
+        ** apply set_add_iff.
+           right.
+           destruct msg as [[c v] j].
+           apply equivocating_sender_add_in_sorted_iff in H_in0. 
+           destruct H_in0.
+           destruct H1; contradiction.
+           assumption.
+      * intros v0 H_in0.
+        destruct (classic (v0 = sender msg)). 
+        ** subst.
+           apply set_add_iff in H_in0.
+           destruct H_in0.
+           apply set_map_in.
+           apply filter_in.
+           apply in_eq. 
+           rewrite equivocating_in_state_correct.
+           red. exists msg'.
+           split. 
+           right; assumption.
+           assumption. contradiction. 
+        ** apply set_add_iff in H_in0.
+           destruct H_in0.
+           contradiction.
+           apply set_map_exists in H1.
+           destruct H1 as [msg0 [H_in0 H_sender0]].
+           apply set_map_exists. exists msg0.
+           split. 2 : assumption.
+           apply filter_in.
+           apply filter_In in H_in0.
+           destruct H_in0.
+           right; assumption.
+           apply filter_In in H_in0.
+           destruct H_in0.
+           rewrite equivocating_in_state_correct.
+           red. rewrite equivocating_in_state_correct in H2.
+           red in H2.
+           destruct H2 as [msg0_partner [H_in0 H_equiv0]].
+           exists msg0_partner.
+           split.
+           right; assumption.
+           assumption. *) 
+Abort.
+
+(* We need some guarantees that the next equivocation state function actually works as intended, abstracting away all the details of add_weight one/two/three. *) 
+Definition add_weight_under `{CBC_protocol_eq_specific} (s : state) (v : validators) :=
+  (fault_weight_state s + proj1_sig (weight v) <= proj1_sig t)%R.
+Class CBC_protocol_eq_more_specific `{CBC_protocol_eq_specific} :=
+  {
+    add_comm : forall s msg1 msg2, state_eq (add_message msg1 (add_message msg2 s)) (add_message msg2 (add_message msg1 s));
+    (* More details about this next state that depends on its implementation, but that we include here after we have defined all the relevant operations *) 
+                           
+    prot_state_not_heavy : forall sigma,
+      prot_state sigma ->
+      not_heavy sigma;
+    (* next_equivocation_state_adds_equivocator :
+      forall j v v',
+        prot_state j -> 
+        v <> v' ->
+        In v (equivocating_senders (next_equivocation_state j v v')); *)
+    next_equivocation_state_adds_equivocators : forall (j : state) (v v' v0 : validators),
+        In v0 (equivocating_senders (next_equivocation_state j v v')) <-> 
+        In v0 (equivocating_senders j) \/ v0 = v; 
+
+    (* This relies on add_weight_one/two/three *) 
+    equivocation_adds_fault_weight :
+      
+      forall (j : state),
+        prot_state j ->
+        forall (v v' : validators),
+          ~ In v (equivocating_senders j) -> 
+          v <> v' ->  
+          fault_weight_state (next_equivocation_state j v v') = 
+          (fault_weight_state j + proj1_sig (weight v))%R;
+
+    (* This relies on the specific construction of the equivocating messages *) 
+    next_equivocation_protocol_state :
+      
+      forall j,
+        prot_state j ->
+        forall v v',
+          ~ In v (equivocating_senders j) -> 
+          v <> v' -> 
+          (add_weight_under j v ->
+           prot_state (next_equivocation_state j v v'));
+
+    (* This relies on the above and is just cleaner *) 
+    next_equivocation_adds_weight :
+      
+      forall (s : state),
+        prot_state s ->
+        forall (v : validators),
+          (* If the weight is not over *) 
+          add_weight_under s v ->
+          (* And the sender is not already equivocating *) 
+          ~ In v (equivocating_senders s) -> 
+          forall (v' : validators),
+            v <> v' ->
+            (* Then we get a protocol state *) 
+            prot_state (next_equivocation_state s v v') /\
+            (* With increased weight *) 
+            fault_weight_state (next_equivocation_state s v v') =
+            (fault_weight_state s + proj1_sig (weight v))%R;
+
+                                                     
+  }.
+
+(* Now I think we are ready to define this recursive equivocation function. *)
+
+Fixpoint next_equivocation_rec' `{CBC_protocol_eq_more_specific} (s : state) (vs : list validators) (v0 : validators) : state :=
+  match vs with
+  | [] => s
+  | hd :: tl => next_equivocation_state (next_equivocation_rec' s tl v0) hd v0
+  end.
+
+Lemma next_equivocations_keeps_messages `{CBC_protocol_eq_more_specific} :
+  forall (s : state) (vs : list validators) (v0 : validators),
+  forall (msg : message),
+    in_state msg s ->
+    in_state msg (next_equivocation_rec' s vs v0). 
+Proof.
+  intros s vs v0 msg H_in.
+  induction vs as [|hd tl IHvs].
+  - assumption.
+  - simpl.
+    apply in_state_correct.
+    apply next_equivocation_state_keeps_messages.
+    now apply in_state_correct in IHvs.
+Qed.
+
+Lemma next_equivocations_equivocating_senders_right `{CBC_protocol_eq_more_specific} :
+  forall (s : state) (vs : list validators) (v0 v : validators),
+    (In v vs -> v <> v0) ->
+    In v (equivocating_senders (next_equivocation_rec' s vs v0)) ->
+    In v vs \/ In v (equivocating_senders s). 
+Proof.
+  rename H into elephant;
+    rename H0 into squirrel.
+  intros s vs; induction vs as [|hd tl IHvs]; intros v0 v H_neq. 
+  - intros. 
+    simpl in H. tauto. 
+  - intros.
+    spec IHvs v0 v.  
+    spec IHvs. 
+    { intros. 
+      spec H_neq. right; assumption.
+      assumption. }
+    simpl in H.
+    apply next_equivocation_state_adds_equivocators in H. 
+    destruct H as [? | ?].
+    spec IHvs H. destruct IHvs.
+    left. right. assumption.
+    tauto. subst. left. left. reflexivity.
+Qed.
+
+Lemma next_equivocations_equivocating_senders_left_weak `{CBC_protocol_eq_more_specific} :
+  forall (s : state) (vs : list validators) (v0 v : validators),
+    prot_state (next_equivocation_rec' s vs v0) -> 
+    (In v vs -> v <> v0) ->
+    In v vs ->
+    In v (equivocating_senders (next_equivocation_rec' s vs v0)). 
+Proof.
+  rename H into elephant; rename H0 into squirrel.
+  intros s vs; induction vs as [|hd tl IHvs]; intros v0 v H_prot H_neq H_in. 
+  - inversion H_in. 
+  - assert (H_prot_sub : prot_state (next_equivocation_rec' s tl v0)).
+    { apply protocol_state_incl with (next_equivocation_rec' s (hd :: tl) v0).
+      assumption.
+      apply prot_state_nodup in H_prot.
+      simpl in H_prot.
+      apply nodup_state_reach with (next_equivocation_state (next_equivocation_rec' s tl v0) hd v0). 
+      assumption.
+      apply next_equivocation_state_incl.
+      simpl. apply next_equivocation_state_incl. }
+    spec IHvs v0 v.
+    spec IHvs H_prot_sub. 
+    spec IHvs. intros. apply H_neq. auto.
+    (* Case analysis on where v is *)
+    destruct H_in as [H_eq | H_in].
+    * (* When we are looking at the hd element, *)
+      subst.
+      simpl.
+      apply next_equivocation_state_adds_equivocators. 
+      tauto. 
+    * spec IHvs H_in.
+      simpl. 
+      assert (H_useful := equivocating_senders_incl). 
+      spec H_useful (next_equivocation_rec' s tl v0) (next_equivocation_state (next_equivocation_rec' s tl v0) hd v0).
+      spec H_useful.
+      apply next_equivocation_state_incl.
+      apply H_useful. assumption.
+Qed.
+
+Lemma next_equivocations_add_weights `{CBC_protocol_eq_more_specific} : 
+  forall (s : state),
+    prot_state s ->
+    forall (vs : list validators) (v0 : validators),
+      NoDup vs -> 
+      (* The sum weight is not over *)
+      (fault_weight_state s + sum_weights vs <= proj1_sig t)%R ->
+      (* None of the senders are already equivocating *) 
+      (forall (v : validators),
+          In v vs -> ~ In v (equivocating_senders s) /\ v <> v0) ->
+      (* Then we end up with a protocol state *)
+      prot_state (next_equivocation_rec' s vs v0) /\
+      (* And s recursively adds the sums of all the weights in vs *) 
+      fault_weight_state (next_equivocation_rec' s vs v0) =
+      (fault_weight_state s + sum_weights vs)%R.
+Proof.
+  rename H into elephant; rename H0 into squirrel.
+  intros s about_s vs v0 H_nodup H_underweight H_disjoint. 
+  induction vs as [|hd tl IHvs].
+  - (* Base case : no validators to add *)
+    split. assumption. 
+    rewrite Rplus_0_r. reflexivity.
+  - (* Induction step *)
+    (* Discharging first premise *)  
+    spec IHvs. 
+    rewrite NoDup_cons_iff in H_nodup; tauto.
+    (* Discharging second premise *)
+    spec IHvs.
+    simpl in H_underweight.
+    apply (Rplus_le_reg_pos_r (fault_weight_state s + sum_weights tl) (proj1_sig (weight hd)) (proj1_sig t)).
+    destruct (weight hd). simpl.
+    apply Rge_le.
+    apply Rgt_ge. assumption. 
+    rewrite Rplus_assoc.
+    rewrite (Rplus_comm (sum_weights tl) (proj1_sig (weight hd))).
+    rewrite <- Rplus_assoc.
+    rewrite <- Rplus_assoc in H_underweight.
+    assumption.
+    (* Discharging third premise *)
+    spec IHvs.
+    intros. spec H_disjoint v. spec H_disjoint. 
+    right; assumption.
+    assumption. 
+    (* Now. *)
+    destruct IHvs as [H_prot H_weight].
+    spec H_disjoint hd (in_eq hd tl).
+    assert (H_notin_tl : ~ In hd tl).
+    { rewrite NoDup_cons_iff in H_nodup.
+      tauto. }
+    destruct H_disjoint as [H_disjoint H_neq].
+    assert (H_rewrite := next_equivocations_equivocating_senders_right s tl v0 hd).
+    spec H_rewrite.
+    intros. assumption.
+    split.
+    + simpl.  
+      apply next_equivocation_protocol_state; try assumption.
+      intros H_absurd.
+      spec H_rewrite H_absurd. 
+      tauto.
+      (* Need a helper lemma about weight adding here *) 
+      unfold add_weight_under.
+      rewrite H_weight. simpl in H_underweight.
+      rewrite <- Rplus_assoc in H_underweight.
+      rewrite Rplus_assoc.
+      rewrite (Rplus_comm (sum_weights tl) (proj1_sig (weight hd))).
+      rewrite <- Rplus_assoc.
+      assumption.
+    + simpl.
+      rewrite (Rplus_comm (proj1_sig (weight hd)) (sum_weights tl)).
+      rewrite <- Rplus_assoc.
+      rewrite <- H_weight.
+      apply equivocation_adds_fault_weight; try assumption.
+      intro H_absurd. spec H_rewrite H_absurd. 
+      tauto. 
+Qed.
+
+Lemma next_equivocations_keeps_equivocating_senders `{CBC_protocol_eq_more_specific} :
+  forall (s : state) (vs : list validators) (v0 : validators),
+  forall (v : validators),
+    In v (equivocating_senders s) ->
+    In v (equivocating_senders (next_equivocation_rec' s vs v0)). 
+Proof.
+  intros s vs v0 v H_in.
+  induction vs as [|hd tl IHvs].
+  - assumption.
+  - simpl.
+    assert (H_useful := next_equivocation_state_keeps_equivocators (next_equivocation_rec' s tl v0) hd v0 v IHvs).
+    assumption.
+Qed.
+
+Definition get_estimate `{CBC_protocol_eq_more_specific} (s : state) :=
+  proj1_sig (choice consensus_values (E s) (estimator_total s)).
+
+Definition get_estimate_correct `{CBC_protocol_eq_more_specific} (s : state) :=
+  proj2_sig (choice consensus_values (E s) (estimator_total s)). 
+
+Definition potentially_pivotal_state `{CBC_protocol_eq_more_specific} (v : validators) (s : state) :=
+  (* We say that v is a pivotal validator for some state s iff : *)
+  (* v is not already equivocating in s *) 
+  ~ In v (equivocating_senders s) /\
+  (* There is a remaining list of validators *) 
+  exists (vs : list validators),
+    (* That is duplicate-free *)
+    NoDup vs /\
+    (* Doesn't contain v *)
+    ~ In v vs /\ 
+    (* That are all not already equivocating in s *) 
+    (forall (v : validators), In v vs -> ~ In v (equivocating_senders s)) /\
+    (* That tip over s's fault weight but only with the help of v *) 
+    (sum_weights ((equivocating_senders s) ++ vs) <= proj1_sig t)%R /\
+    (sum_weights ((equivocating_senders s) ++ vs) >
+     proj1_sig t - proj1_sig (weight v))%R. 
+
+Lemma pivotal_validator_extension `{CBC_protocol_eq_more_specific} : forall (vsfix vss : list validators),
+  NoDup vsfix ->
+  (* and whose added weight does not pass the threshold *)
+  (sum_weights vsfix <= proj1_sig t)%R ->
+  NoDup (vss ++ vsfix) ->
+  (sum_weights (vss ++ vsfix) > proj1_sig t)%R ->
+  exists (vs : list validators),
+    NoDup vs /\
+    incl vs vss /\
+    (sum_weights (vs ++ vsfix) > proj1_sig t)%R /\
+    exists (v : validators),
+      In v vs /\
+      (sum_weights ((set_remove  (@compare_eq_dec validators compare (@compare_strictorder validators about_validators)) v vs) ++ vsfix) <= proj1_sig t)%R.
+Proof.
+  rename H into elephant;
+    rename H0 into squirrel;
+    rename H1 into bunny.
+  destruct t as [t about_t]; simpl in *.
+  intro.
+  induction vss; intros.
+  - simpl in H2. exfalso. apply (Rge_gt_trans t) in H2; try (apply Rle_ge; assumption).
+    apply Rgt_not_eq in H2. apply H2. reflexivity.
+  - simpl in H2. destruct (Rtotal_le_gt (sum_weights (vss ++ vsfix)) t).
+    + exists (a :: vss). repeat split; try assumption.
+      * apply append_nodup_left in H1. assumption.
+      * apply incl_refl.
+      * exists a. split; try (left; reflexivity).
+        simpl. rewrite eq_dec_if_true; try reflexivity. assumption.
+    + simpl in H1. apply NoDup_cons_iff in H1. destruct H1 as [Hnin Hvss]. apply IHvss in H3; try assumption.
+      destruct H3 as [vs [Hvs [Hincl Hex]]].
+      exists vs. repeat (split;try assumption). apply incl_tl. assumption.
+Qed.
+
+Lemma sum_weights_app `{CBC_protocol_eq_more_specific} : forall vs vs',
+  sum_weights (vs ++ vs') = (sum_weights vs + sum_weights vs')%R.
+Proof.
+  induction vs; intros; simpl.
+  - rewrite Rplus_0_l. reflexivity.
+  - rewrite IHvs. rewrite Rplus_assoc. reflexivity.
+Qed.
+
+(* This is a critical lemma *) 
+Lemma all_pivotal_validator `{CBC_protocol_eq_more_specific} :
+  forall (s : state),
+    prot_state s -> 
+  exists (v : validators),
+    potentially_pivotal_state v s. 
+Proof.
+  rename H into elephant;
+    rename H0 into squirrel;
+    rename H1 into bunny.
+  intros s about_s.
+  destruct suff_val as [vs [Hvs Hweight]].
+  remember (equivocating_senders s) as eqv_s.
+  remember (set_diff (@compare_eq_dec validators (@compare validators about_validators) (@compare_strictorder validators about_validators)) vs eqv_s) as vss.
+  assert (sum_weights (vss ++ eqv_s) > proj1_sig t)%R.
+  { apply Rge_gt_trans with (sum_weights vs); try assumption.
+    apply Rle_ge. apply sum_weights_incl; try assumption.
+    - rewrite Heqvss. apply diff_app_nodup; try assumption.
+      subst. unfold equivocating_senders. apply set_map_nodup.
+    - rewrite Heqvss. intros a Hin. apply in_app_iff.
+      rewrite set_diff_iff. apply or_and_distr_left.
+      split; try (left; assumption).
+      destruct (in_dec (@compare_eq_dec validators (@compare validators about_validators) (@compare_strictorder validators about_validators)) a eqv_s); (left; assumption) || (right; assumption).
+  }
+  apply pivotal_validator_extension in H. 
+  - destruct H as [vs' [Hnodup_vs' [Hincl_vs' [Hgt [v [Hin_v Hlt]]]]]].
+    exists v. split.
+    + subst. apply Hincl_vs' in Hin_v. apply set_diff_elim2 in Hin_v. assumption.
+    + exists (set_remove (@compare_eq_dec validators compare (@compare_strictorder validators about_validators)) v vs').
+      assert (NoDup (set_remove (@compare_eq_dec validators compare (@compare_strictorder validators about_validators)) v vs')) as Hnodup_remove
+      ; try apply set_remove_nodup; try assumption.
+      repeat split.
+      * assumption.
+      * try apply set_remove_elim; try assumption.
+      * intros. apply set_remove_1 in H. apply Hincl_vs' in H. subst.
+        apply set_diff_elim2 in H. assumption.
+      * subst. rewrite sum_weights_app in *. rewrite Rplus_comm in Hlt.
+        assumption.
+      * apply Rlt_gt. apply Rplus_lt_reg_r with (proj1_sig (weight v)).
+        unfold Rminus. rewrite Rplus_assoc. rewrite Rplus_opp_l.
+        rewrite Rplus_0_r. apply Rgt_lt.
+        apply Rge_gt_trans with (sum_weights (vs' ++ eqv_s)); try assumption.
+        unfold Rge. right. rewrite Rplus_comm.
+        rewrite sum_weights_app. rewrite (Rplus_comm (sum_weights (equivocating_senders s))) .
+        rewrite <- Rplus_assoc. rewrite sum_weights_app. subst.
+        apply Rplus_eq_compat_r.
+        symmetry. apply sum_weights_in; try assumption.
+  - subst. apply set_map_nodup.
+  - subst. apply prot_state_not_heavy. assumption.
+  - subst. apply diff_app_nodup; try assumption.
+    apply set_map_nodup.
+Qed.
+
+(* Defining reachablity in terms of message sending *)
+Definition in_future `{CBC_protocol_eq_more_specific} (s1 s2 : state) :=
+  reach s1 s2. 
+
+Definition next_future `{CBC_protocol_eq_more_specific} (s1 s2 : state) :=
+   exists (msg : message), state_eq (add_message msg s1) s2. 
+
+Definition in_past `{CBC_protocol_eq_more_specific} (s1 s2 : state) :=
+  reach s2 s1. 
+
+Definition no_common_future `{CBC_protocol_eq_more_specific} (s1 s2 : pstate_light) :=
+  forall (s : pstate_light), in_future s1 s /\ in_future s2 s -> False. 
+
+Definition yes_common_future `{CBC_protocol_eq_more_specific} (s1 s2 : pstate_light) :=
+  exists (s : pstate_light), in_future s1 s /\ in_future s2 s. 
+
+Definition strong_nontriviality `{CBC_protocol_eq_more_specific} :=
+  (* For every state, there exists a state *) 
+  forall (s1 : pstate_light),
+  exists (s2 : pstate_light),
+    (* That is reachable in one step *) 
+    next_future s1 s2 /\
+    (* And there exists a third state *)
+    exists (s3 : pstate_light),
+      (* Such that s1 and s3 share a common future *)
+      yes_common_future s1 s3
+      /\
+      (* But s2 and s3 don't. *) 
+      no_common_future s2 s3.
+
+Lemma distinct_sender_total `{CBC_protocol_eq_more_specific} : forall v1 : validators, exists v2 : validators, v1 <> v2.
+Proof.
+  intros.
+  destruct two_senders  as [v1' [v2' Hneq]].
+  destruct ((@compare_eq_dec validators compare (@compare_strictorder validators about_validators)) v1 v1') eqn:Heq.
+  - subst. exists v2'. assumption.
+  - exists v1'. assumption.
+Qed.
+
+Definition get_distinct_sender `{CBC_protocol_eq_more_specific} (v : validators) :=
+  proj1_sig (choice validators (fun v' => v <> v') (distinct_sender_total v)).
+
+Definition get_distinct_sender_correct `{CBC_protocol_eq_more_specific} (v : validators) :=
+  proj2_sig (choice validators (fun v' => v <> v') (distinct_sender_total v)).
+
+Lemma get_distinct_sender_correct' `{CBC_protocol_eq_more_specific} :
+  forall v, get_distinct_sender v <> v. 
+Proof.
+  intros. unfold get_distinct_sender.
+  assert (H_useful := get_distinct_sender_correct v).
+  simpl in *.
+  intro H_absurd.
+  apply H_useful; symmetry; assumption.
+Qed.
+
+Theorem strong_nontriviality_full `{CBC_protocol_eq_more_specific} : strong_nontriviality.  
+Proof.
+  rename H into elephant;
+    rename H0 into squirrel;
+    rename H1 into bunny. 
+  intros [s1 about_s1]. 
+  destruct (all_pivotal_validator s1 about_s1) as [v [H_v [vs [H_nodup [H_v_notin [H_disjoint [H_under H_over]]]]]]].
+  (* Now we need to construct s2 in a smarter way *)
+  (* v could potentially equivocate, but we don't want to go so far. *) 
+  assert (H_overkill := next_equivocation_state_horn s1 v (get_distinct_sender v)).
+  destruct H_overkill as [msg1 [msg2 [msg3 [H_eq [H_equiv [H_sender1 [H_sender2 [H_justi H_prot]]]]]]]]. 
+  remember (add_message msg3 s1) as s2.
+  assert (about_s2 : prot_state s2) by (subst; tauto).
+  (* Book-keeping *)
+  assert (H_s1_s2_senders : set_eq (equivocating_senders s1) (equivocating_senders (s2))) by admit. 
+  assert (H_s1_s2_weight : fault_weight_state s1 = fault_weight_state (s2)) by admit. 
+  exists (exist prot_state s2 about_s2).
+  split.
+  (* Proving that s2 is a next state is trivial *)
+  exists msg3. subst. 
+  simpl. apply Equivalence_Reflexive.
+  (* Now we need to construct s3. *)
+  (* First we add the equivocating partner message *) 
+  remember (add_message msg2 (add_message msg1 s1)) as s1'.
+  assert (about_s1' : prot_state s1') by (subst; tauto).
+  (* Book-keeping step *) 
+  assert (H_eq_senders : set_eq (equivocating_senders s1') (equivocating_senders s1)) by admit.
+  assert (H_s_inter_weight : fault_weight_state s1' = fault_weight_state s1).
+  { apply equivocating_senders_fault_weight_eq; assumption. }
+  (* Now we are ready to construct s3 from s1' *)
+  (* And if we have set up everything correctly, the premises at this point in the proof are sufficient. *)
+  remember (next_equivocation_rec' s1' vs v) as s3.
+  assert (about_s3 : prot_state s3).
+  { rewrite Heqs3. apply next_equivocations_add_weights.
+    { subst.
+      tauto. }
+    assumption. 
+    rewrite H_s_inter_weight. rewrite sum_weights_app in H_under.
+    assumption. 
+    intros. spec H_disjoint v0 H.
+    destruct H_eq_senders as [H_left H_right].
+    spec H_right v0.
+    split. intro H_absurd. spec H_left v0 H_absurd.
+    contradiction. intro H_absurd. subst. contradiction. } 
+  exists (exist prot_state s3 about_s3).
+  repeat split.
+  exists (exist prot_state s3 about_s3). split.
+  subst. simpl.
+  red.
+  admit. 
+
+  apply reach_refl.
+  red. intros [s about_s] H.   
+  destruct H as [H_in2 H_in3].
+  assert (H_in2_copy := H_in2);
+    assert (H_in3_copy := H_in3).  
+  (* Now we show that two equivocating messages are in s *)
+  (* First message *) 
+  simpl in *.
+  assert (H_in2' := in_state_morphism s2 s H_in2 msg3).
+  spec H_in2'. 
+  subst.
+  apply add_message_in_state. 
+  (* Second message *) 
+  assert (H_in3' := in_state_morphism s3 s H_in3 msg2).
+  spec H_in3'.
+  subst.
+  admit. 
+  (* Now we say that v will be an equivocating sender inside s *)
+  assert (H_v_in : In v (equivocating_senders s)).
+  { apply equivocating_senders_correct.
+    exists msg2. 
+    repeat split; try assumption.
+    exists msg3.
+    split; try tauto.
+    apply equivocating_messages_correct.
+    assumption. }
+  clear H_in2 H_in3 H_equiv. 
+  (* Now we say that v's weight will be inside s's fault weight *)
+  (* This part is a little tricky *)
+  assert (H_equivocators_s : incl ((v :: (equivocating_senders s2) ++ vs)) (equivocating_senders s)). 
+  { intros v0 H_in0.
+    destruct H_in0 as [H_hd | H_tl].
+    + subst. assumption.
+    + apply in_app_iff in H_tl.
+      destruct H_tl as [H_left | H_right].
+      * eapply equivocating_senders_incl.
+        apply H_in2_copy.
+        assumption.
+        * assert (H_in_v0 : In v0 (equivocating_senders (next_equivocation_rec' s1' vs v))).
+          { apply next_equivocations_equivocating_senders_left_weak. 
+            subst. assumption. intros.
+            2 : assumption.
+            intro H_absurd; subst; contradiction. } 
+          rewrite <- Heqs3 in H_in_v0.
+          eapply equivocating_senders_incl.
+          exact H_in3_copy. 
+          assumption.
+    }
+    assert (H_s_overweight : (proj1_sig (weight v) + fault_weight_state (s2) + sum_weights vs <= fault_weight_state s)%R). 
+    { replace ((proj1_sig (weight v) + fault_weight_state (s2) + sum_weights vs))%R with (sum_weights ([v] ++ (equivocating_senders (s2)) ++ vs)).
+      apply sum_weights_incl.
+      { (* Proving mutual NoDup *) 
+        apply nodup_append.
+        apply NoDup_cons. intros; inversion 1.
+        constructor.
+        apply nodup_append.
+        apply set_map_nodup. assumption.
+        { intros. intro Habsurd. spec H_disjoint a Habsurd.
+          destruct H_s1_s2_senders as [_ H_useful].
+          spec H_useful a H. contradiction.
+        }
+        { intros. intro Habsurd. spec H_disjoint a H.
+          destruct H_s1_s2_senders as [_ H_useful].
+          spec H_useful a Habsurd. contradiction. }
+        { intros. inversion H. intro Habsurd.
+          apply in_app_iff in Habsurd. destruct Habsurd.
+          destruct H_s1_s2_senders as [_ H_useful];
+            spec H_useful a H1.
+          subst; contradiction. subst; contradiction. inversion H0. } 
+        { intros. intro Habsurd.
+          inversion Habsurd.
+          apply in_app_iff in H. destruct H.
+          destruct H_s1_s2_senders as [_ H_useful];
+            spec H_useful a H.
+          subst; contradiction. subst; contradiction. inversion H0. } 
+      }
+      apply set_map_nodup. assumption.
+      do 2 rewrite sum_weights_app.
+      unfold fault_weight_state.
+      simpl. ring. }
+    apply prot_state_not_heavy in about_s.
+    red in about_s.
+    assert (H_finale := Rle_trans _ _ _ H_s_overweight about_s). auto.
+    rewrite sum_weights_app in H_over.
+    unfold fault_weight_state in H_s1_s2_weight at 1. 
+    rewrite H_s1_s2_weight in H_over.
+    apply (Rplus_gt_compat_l (proj1_sig (weight v))) in H_over. 
+    replace (proj1_sig (weight v) + (proj1_sig t - proj1_sig (weight v)))%R with (proj1_sig t)%R in H_over by ring.
+    rewrite <- Rplus_assoc in H_over. 
+    apply Rgt_not_le in H_over.
+    contradiction.
+Admitted. 
+
+
+
+Definition next_future `{CBC_protocol_eq_specific} (s1 s2 : state) :=
+   exists (msg : message), state_eq (add_message msg s1) s2. 
+
+Definition pstate `{CBC_protocol_eq_specific} : Type :=
+  { s : state | prot_state s}.
+
+Definition pstate_proj1 `{CBC_protocol_eq_specific} (ps : pstate) :=
+  proj1_sig ps. 
+
+Coercion pstate_proj1 : pstate >-> state. 
+
+Definition no_common_future `{CBC_protocol_eq_specific} (s1 s2 : pstate) :=
+  forall (s : pstate), reach s1 s /\ reach s2 s -> False. 
+
+Definition yes_common_future `{CBC_protocol_eq_specific} (s1 s2 : pstate) :=
+  exists (s : pstate), reach s1 s /\ reach s2 s. 
+
+Definition strong_nontriviality `{CBC_protocol_eq_specific} :=
+  (* For every state, there exists a state *) 
+  forall (s1 : pstate),
+  exists (s2 : pstate),
+    (* That is reachable in one step *) 
+    next_future s1 s2 /\
+    (* And there exists a third state *)
+    exists (s3 : pstate),
+      (* Such that s1 and s3 share a common future *)
+      yes_common_future s1 s3
+      /\
+      (* But s2 and s3 don't. *) 
+      no_common_future s2 s3.
+
+Theorem strong_nontriviality_full `{CBC_protocol_eq_specific} : strong_nontriviality.  
+Proof.
+  intros [s1 about_s1]. 
+  destruct (all_pivotal_validator s1 about_s1) as [v [H_v [vs [H_nodup [H_v_notin [H_disjoint [H_under H_over]]]]]]].
+  remember (exist protocol_state ((get_estimate s1,v,hash_state s1) :: s1) (copy_protocol_state s1 about_s1  v)) as s2. 
+  (* Book-keeping *)
+  assert (H_s1_s2_senders : set_eq (equivocating_senders s1) (equivocating_senders (proj1_sig s2))) by (subst; apply equivocating_senders_sorted_extend). 
+  assert (H_s1_s2_weight : fault_weight_state s1 = fault_weight_state (proj1_sig s2)) by (subst; apply add_weight_one). 
+  exists s2.
+  (* Proving next-step relation is trivial. *) 
+  split.
+  exists (get_estimate s1,v,hash_state s1); subst; simpl in *.
+  split; intros x H_in.
+  rewrite set_add_iff in H_in. destruct H_in. subst. apply in_eq.
+  right; tauto.
+  inversion H_in; subst; rewrite set_add_iff; tauto.
+  (* s3 is the state with equivocations from all the senders in vs recursively added to s1, in addition to (c,v,s1)'s equivocating partner message. *)
+  (* First we add the equivocating partner message *)
+  remember ((get_estimate ((get_estimate s1, get_distinct_sender v, hash_state s1) :: s1), v, hash_state ((get_estimate s1, get_distinct_sender v, hash_state s1) :: s1)) :: ((get_estimate s1, get_distinct_sender v, hash_state s1) :: s1)) as s1'.
+  (* Book-keeping step *) 
+  assert (H_eq_senders : set_eq (equivocating_senders s1') (equivocating_senders s1)).
+  { subst. 
+    assert (H_useful := equivocating_senders_sorted_extend ((get_estimate s1, get_distinct_sender v, hash_state s1) :: s1) v).
+    eapply set_eq_tran.
+    apply set_eq_comm. exact H_useful.
+    apply set_eq_comm. apply equivocating_senders_sorted_extend. }
+  assert (H_s_inter_weight : fault_weight_state s1' = fault_weight_state s1).
+  { apply equivocating_senders_fault_weight_eq; assumption. }
+  (* Now we are ready to construct s3 from s1' *)
+  (* And if we have set up everything correctly, the premises at this point in the proof are sufficient. *)
+  remember (next_equivocation_rec' s1' vs v) as s3.
+  assert (about_s3 : protocol_state s3).
+  { rewrite Heqs3. apply next_equivocations_add_weights.
+    { subst.
+      apply copy_protocol_state; try apply get_estimate_correct; try assumption. 
+      apply copy_protocol_state; try apply get_estimate_correct; try assumption. } 
+    assumption.
+    rewrite H_s_inter_weight. rewrite sum_weights_app in H_under.
+    assumption. 
+    intros. spec H_disjoint v0 H.
+    destruct H_eq_senders as [H_left H_right].
+    spec H_right v0.
+    split. intro H_absurd. spec H_left v0 H_absurd.
+    contradiction. intro H_absurd. subst. contradiction. } 
+  exists (exist protocol_state s3 about_s3).
+  repeat split.
+  - (* Proving that s1 and s3 share a common future *)
+    red. exists (exist protocol_state s3 about_s3).
+    split. simpl. red.
+    red. subst.
+    intros m0 H_in.
+    (* Need to prove that next_equivocation_rec' doesn't drop messages *) 
+    apply next_equivocations_keeps_messages.
+    do 2 right. 
+    assumption. 
+    apply incl_refl.
+  - (* Proving that s2 and s3 don't share a common future *)
+    (* Arbitrary state in both s2 and s3 leads to a contradiction *) 
+    red. intros [s about_s] H.   
+    destruct H as [H_in2 H_in3].
+    assert (H_in2_copy := H_in2);
+      assert (H_in3_copy := H_in3).  
+    (* Now we show that two equivocating messages are in s *)
+    (* First message *) 
+    spec H_in2 (get_estimate s1,v,hash_state s1).
+    spec H_in2. 
+    subst. 
+    apply in_eq. 
+    (* Second message *) 
+    spec H_in3 (get_estimate
+                ((get_estimate s1, get_distinct_sender v, hash_state s1) :: s1), v,
+             
+               hash_state ((get_estimate s1, get_distinct_sender v, hash_state s1) ::  s1)).
+    spec H_in3.
+    { (* Proving that this message is in s3 *)
+      assert (H_obv : In (get_estimate ((get_estimate s1, get_distinct_sender v, hash_state s1) ::  s1), v, hash_state ((get_estimate s1, get_distinct_sender v, hash_state s1) ::  s1)) s1').
+      { subst. 
+        left. reflexivity. }
+      apply (next_equivocations_keeps_messages s1' vs v) in H_obv.
+      subst; assumption. }
+    (* Now we prove that these two messages are equivocating *) 
+    simpl in *.
+    assert (H_equiv : equivocating_messages_prop (get_estimate s1,v,hash_state s1)
+                                                 (get_estimate ((get_estimate s1, get_distinct_sender v, hash_state s1) :: s1), v, hash_state ((get_estimate s1, get_distinct_sender v, hash_state s1) :: s1))).
+    apply about_equivocating_messages. 
+    assumption. apply get_distinct_sender_correct. 
+    (* Now we say that v will be an equivocating sender inside s *)
+    assert (H_v_in : In v (equivocating_senders s)).
+    { apply equivocating_senders_correct.
+      exists (get_estimate s1, v, hash_state s1). 
+      repeat split; try assumption.
+      exists (get_estimate ((get_estimate s1, get_distinct_sender v, hash_state s1) :: s1), v, hash_state ( (get_estimate s1, get_distinct_sender v, hash_state s1) :: s1)).
+      split. assumption. assumption. }
+    clear H_in2 H_in3 H_equiv. 
+    (* Now we say that v's weight will be inside s's fault weight *)
+    (* This part is a little tricky *)
+    assert (H_equivocators_s : incl (v :: (equivocating_senders (proj1_sig s2) ++ vs)) (equivocating_senders s)). 
+    { intros v0 H_in0.
+      destruct H_in0 as [H_hd | H_tl].
+      + subst. assumption.
+      + apply in_app_iff in H_tl.
+        destruct H_tl as [H_left | H_right].
+        * eapply equivocating_senders_incl.
+          apply H_in2_copy.
+          assumption.
+        * assert (H_in_v0 : In v0 (equivocating_senders (next_equivocation_rec' s1' vs v))).
+          { apply next_equivocations_equivocating_senders_left_weak. 
+            subst; assumption. intros.
+            2 : assumption.
+            intro H_absurd; subst; contradiction. } 
+          rewrite <- Heqs3 in H_in_v0.
+          eapply equivocating_senders_incl.
+          exact H_in3_copy. 
+          assumption.
+    }
+    assert (H_s_overweight : (proj1_sig (weight v) + fault_weight_state (proj1_sig s2) + sum_weights vs <= fault_weight_state s)%R). 
+    { replace ((proj1_sig (weight v) + fault_weight_state (proj1_sig s2) + sum_weights vs))%R with (sum_weights ([v] ++ (equivocating_senders (proj1_sig s2)) ++ vs)).
+      apply sum_weights_incl.
+      { (* Proving mutual NoDup *) 
+        apply nodup_append.
+        apply NoDup_cons. intros; inversion 1.
+        constructor.
+        apply nodup_append.
+        apply set_map_nodup. assumption.
+        { intros. intro Habsurd. spec H_disjoint a Habsurd.
+          destruct H_s1_s2_senders as [_ H_useful].
+          spec H_useful a H. contradiction.
+        }
+        { intros. intro Habsurd. spec H_disjoint a H.
+          destruct H_s1_s2_senders as [_ H_useful].
+          spec H_useful a Habsurd. contradiction. }
+        { intros. inversion H. intro Habsurd.
+          apply in_app_iff in Habsurd. destruct Habsurd.
+          destruct H_s1_s2_senders as [_ H_useful];
+            spec H_useful a H1.
+          subst; contradiction. subst; contradiction. inversion H0. } 
+        { intros. intro Habsurd.
+          inversion Habsurd.
+          apply in_app_iff in H. destruct H.
+          destruct H_s1_s2_senders as [_ H_useful];
+            spec H_useful a H.
+          subst; contradiction. subst; contradiction. inversion H0. } 
+      }
+      apply set_map_nodup. assumption.
+      do 2 rewrite sum_weights_app.
+      unfold fault_weight_state.
+      simpl. ring. }
+    apply protocol_state_not_heavy in about_s.
+    red in about_s.
+    assert (H_finale := Rle_trans _ _ _ H_s_overweight about_s). auto.
+    clear -H_finale H_over H_s1_s2_weight.
+    rewrite sum_weights_app in H_over.
+    unfold fault_weight_state in H_s1_s2_weight at 1. 
+    rewrite H_s1_s2_weight in H_over.
+    apply (Rplus_gt_compat_l (proj1_sig (weight v))) in H_over. 
+    replace (proj1_sig (weight v) + (proj1_sig t_full - proj1_sig (weight v)))%R with (proj1_sig t_full)%R in H_over by ring.
+    rewrite <- Rplus_assoc in H_over. 
+    apply Rgt_not_le in H_over.
+    contradiction.
+Qed. 
+
 
 (*
 Class CBC_protocol :=
